progress_bisim

pancake/semantics/proofs/panItreeSemEquivScript.sml
@@ -3128,15 +3128,15 @@ QED
 
 Theorem ltree_Ret_to_evaluate':
     good_dimindex (:α) ∧
-    ltree_lift query_oracle (t:('a,'b)state).ffi (mrec_sem (h_prog (prog,unclock s))) ≈
+    ltree_lift query_oracle (t:('a,'b)state).ffi (mrec_sem (h_prog (prog,s))) ≈
                Ret (r,s')
-    ∧ (s:('a,'b)state).ffi = t.ffi ⇒
-    ∃k k'. evaluate (prog,s with clock := k) = (r,reclock s' with clock := k')
+    ∧ (s:('a,'b)bstate).ffi = t.ffi ⇒
+    ∃k k'. evaluate (prog, reclock s with clock := k) = (r,reclock s' with clock := k')
            ∧ r ≠ SOME TimeOut ∧ k' ≤ k
 Proof
   rpt strip_tac>>
   drule ltree_Ret_to_evaluate>>
-  disch_then $ qspecl_then [‘unclock s’,‘r’,‘s'’,‘prog’] assume_tac>>
+  disch_then $ qspecl_then [‘s’,‘r’,‘s'’,‘prog’] assume_tac>>
   gvs[]>>metis_tac[]
 QED
 
@@ -3150,920 +3150,59 @@ Proof
   fs[LFINITE_fromList,LAPPEND11_FINITE1]>>metis_tac[]
 QED
 
-Theorem stree_trace_Ret_finite:
-  LFINITE (stree_trace query_oracle event_filter s.ffi
-                       (to_stree (mrec_sem (h_prog (prog,s))))) ⇒
-  ∃p. ltree_lift query_oracle s.ffi (mrec_sem (h_prog (prog,s))) ≈ Ret p
-Proof
-  strip_tac>>
-  Cases_on 
-QED
-
-Theorem stree_trace_nonret_infinite:
-  ∀p. ¬ (ltree_lift query_oracle s.ffi (mrec_sem (h_prog (prog,s))) ≈ Ret p) ⇒
-      ¬(LFINITE (stree_trace query_oracle event_filter s.ffi
-                       (to_stree (mrec_sem (h_prog (prog,s))))))
-Proof
-  cheat
-QED
-
 Theorem nonret_imp_timeout:
-  (∀p. ¬(ltree_lift query_oracle s.ffi (mrec_sem (h_prog (prog:'a prog,unclock s))) ≈ Ret p)) ∧
-  good_dimindex (:'a) ⇒
-  ∃r. (evaluate (prog,s)) = (SOME TimeOut,r)
+  ∀s r s' prog:'a prog k.
+    good_dimindex (:α) ∧
+    (∀p. ¬(ltree_lift query_oracle s.ffi (mrec_sem (h_prog (prog,s))) ≈ Ret p)) ⇒
+    ∃s'. evaluate (prog,reclock s with clock := k) = (SOME TimeOut,s')
 Proof
-  CCONTR_TAC>>
-  fs[]>>
-  last_x_assum irule>>
-  rpt (pop_assum mp_tac)>>
-  MAP_EVERY qid_spec_tac [‘s’,‘prog’]>>
-  recInduct evaluate_ind>>rw[]>>
-  fs[Once evaluate_def]>>
-  TRY (fs[h_prog_def,mrec_sem_simps,ltree_lift_cases]>>
-       fs[Once itree_wbisim_cases]>>NO_TAC)
-  >- (gvs[AllCaseEqs(),h_prog_def,h_prog_rule_dec_def,
-          panPropsTheory.eval_upd_clock_eq]>>
-      CASE_TAC>>
-      fs[mrec_sem_simps,ltree_lift_cases,msem_lift_monad_law,ltree_lift_monad_law]>>
-      TRY (fs[Once itree_wbisim_cases]>>NO_TAC)>>
-      pairarg_tac>>gvs[]>>
-      imp_res_tac ltree_wbisim_bind_conv>>
-      qmatch_goalsub_abbrev_tac ‘_ >>= Y’>>
-      first_x_assum $ qspec_then ‘Y’ assume_tac>>
-      irule_at Any itree_wbisim_trans>>
-      first_x_assum $ irule_at Any>>
-      fs[Abbr‘Y’]>>
-      Cases_on ‘p’>>
-      imp_res_tac ltree_lift_state_lift'>>
-      fs[mrec_sem_simps,ltree_lift_cases]>>
-      fs[Once itree_wbisim_cases])
-  >- (gvs[AllCaseEqs(),h_prog_rule_assign_def,h_prog_def,
-          panPropsTheory.eval_upd_clock_eq]>>
-      CASE_TAC>>
-      fs[mrec_sem_simps,ltree_lift_cases,msem_lift_monad_law,ltree_lift_monad_law]>>
-      TRY (fs[Once itree_wbisim_cases]>>NO_TAC)>>
-      IF_CASES_TAC>>
-      gvs[mrec_sem_simps,ltree_lift_cases]>>
-      fs[Once itree_wbisim_cases])
-  >- (gvs[AllCaseEqs(),h_prog_rule_store_def,h_prog_def,
-          panPropsTheory.eval_upd_clock_eq]>>
-      rpt FULL_CASE_TAC>>
-      fs[mrec_sem_simps,ltree_lift_cases,msem_lift_monad_law,ltree_lift_monad_law]>>
-      fs[Once itree_wbisim_cases])
-  >- (gvs[AllCaseEqs(),h_prog_rule_store_byte_def,h_prog_def,
-          panPropsTheory.eval_upd_clock_eq]>>
-      rpt FULL_CASE_TAC>>
-      fs[mrec_sem_simps,ltree_lift_cases,msem_lift_monad_law,ltree_lift_monad_law]>>
-      fs[Once itree_wbisim_cases])
-  >- (Cases_on ‘op’>>
-      gvs[AllCaseEqs(),h_prog_rule_sh_mem_def,h_prog_def,
-          panPropsTheory.eval_upd_clock_eq]>>
-      fs[h_prog_rule_sh_mem_load_def,h_prog_rule_sh_mem_store_def,
-         h_prog_rule_sh_mem_op_def]>>
-      rpt FULL_CASE_TAC>>
-      fs[mrec_sem_simps,ltree_lift_cases,msem_lift_monad_law,ltree_lift_monad_law]>>
-      TRY (pairarg_tac>>fs[])>>
-      fs[Once itree_wbisim_cases])
-  >- (gvs[h_prog_rule_seq_def,h_prog_def,
-          panPropsTheory.eval_upd_clock_eq]>>
-      rpt (pairarg_tac>>fs[])>>
-      fs[mrec_sem_simps,ltree_lift_cases,msem_lift_monad_law,ltree_lift_monad_law]>>
-      Cases_on ‘res’>>fs[]
-      (* res = NONE *)
-      >- (drule ltree_wbisim_bind_conv>>strip_tac>>gvs[]>>
-          qmatch_goalsub_abbrev_tac ‘_ >>= Y’>>
-          first_x_assum $ qspec_then ‘Y’ assume_tac>>
-          irule_at Any itree_wbisim_trans>>
-          first_x_assum $ irule_at Any>>
-          qmatch_asmsub_abbrev_tac ‘Ret pp’>>
-          Cases_on ‘pp’>>
-          imp_res_tac ltree_lift_state_lift'>>
-          fs[Abbr‘Y’]>>
-          fs[mrec_sem_simps,ltree_lift_cases]>>
-          CASE_TAC>>
-          gvs[mrec_sem_simps,ltree_lift_cases]>>
-          TRY (fs[Once itree_wbisim_cases]>>NO_TAC)>>
-          drule_then drule ltree_lift_corres_evaluate>>strip_tac>>gvs[]>>
-          drule_then rev_drule wbisim_Ret_unique>>strip_tac>>gvs[]>>
-          metis_tac[])>>
-      Cases_on ‘p’>>
-      reverse (Cases_on ‘x = Error’)
-      >- (drule_then drule ltree_lift_corres_evaluate>>strip_tac>>gvs[]>>
-          drule_then rev_drule wbisim_Ret_unique>>strip_tac>>gvs[]>>
-
-          drule ltree_wbisim_bind_conv>>strip_tac>>gvs[]>>
-          qmatch_goalsub_abbrev_tac ‘_ >>= Y’>>
-          first_x_assum $ qspec_then ‘Y’ assume_tac>>
-          irule_at Any itree_wbisim_trans>>
-          first_x_assum $ irule_at Any>>
-          fs[Abbr‘Y’]>>
-          gvs[mrec_sem_simps,ltree_lift_cases]>>
-          imp_res_tac ltree_lift_state_lift'>>gvs[]>>
-          fs[Once itree_wbisim_cases])>>
-      gvs[]>>
-      drule_then drule ltree_lift_corres_evaluate_error>>
-      strip_tac>>gvs[]>>
-      drule_then rev_drule wbisim_Ret_unique>>strip_tac>>gvs[]>>
-      drule ltree_wbisim_bind_conv>>strip_tac>>gvs[]>>
-      qmatch_goalsub_abbrev_tac ‘_ >>= Y’>>
-      first_x_assum $ qspec_then ‘Y’ assume_tac>>
-      irule_at Any itree_wbisim_trans>>
-      first_x_assum $ irule_at Any>>
-      fs[Abbr‘Y’]>>
-      gvs[mrec_sem_simps,ltree_lift_cases]>>
-      fs[Once itree_wbisim_cases])
-  (* If *)
-  >- (gvs[AllCaseEqs(),h_prog_rule_cond_def,h_prog_def,
-          panPropsTheory.eval_upd_clock_eq]>>
-      CASE_TAC>>
-      fs[mrec_sem_simps,ltree_lift_cases,
-         msem_lift_monad_law,ltree_lift_monad_law]>>
-      TRY (fs[Once itree_wbisim_cases]>>NO_TAC)>>
-      rpt CASE_TAC>>
-      gvs[mrec_sem_simps,ltree_lift_cases]>>
-      TRY (fs[Once itree_wbisim_cases]>>NO_TAC)>>
-      metis_tac[])
-  (* While *)
-  >- (simp[Once mrec_sem_while_unfold,
-           panPropsTheory.eval_upd_clock_eq]>>
-      CASE_TAC>>
-      fs[mrec_sem_simps,ltree_lift_cases]>>
-      TRY (fs[Once itree_wbisim_cases]>>NO_TAC)>>
-      rpt CASE_TAC>>
-      fs[mrec_sem_simps,ltree_lift_cases]>>
-      TRY (fs[Once itree_wbisim_cases]>>NO_TAC)>>
-      FULL_CASE_TAC>>gvs[]>>
-      rpt (pairarg_tac>>gvs[])>>
-      ‘∀x. (dec_clock x).ffi = x.ffi’ by simp[dec_clock_def]>>fs[]>>
-      drule_then rev_drule ltree_lift_corres_evaluate>>
-      strip_tac>>gvs[]>>
-      Cases_on ‘res’>>fs[ltree_lift_monad_law]
-      (* res = NONE *)
-      >- (drule ltree_wbisim_bind_conv>>strip_tac>>gvs[]>>
-          qmatch_goalsub_abbrev_tac ‘_ >>= Y’>>
-          first_x_assum $ qspec_then ‘Y’ assume_tac>>
-          irule_at Any itree_wbisim_trans>>
-          first_x_assum $ irule_at Any>>
-          imp_res_tac ltree_lift_state_lift'>>gvs[]>>
-          fs[Abbr‘Y’]>>
-          fs[mrec_sem_simps,ltree_lift_cases]>>
-          first_x_assum $ irule>>
-          gvs[Once evaluate_def])>>
-      rename1 ‘Ret (SOME x,_)’>>
-      Cases_on ‘x’>>gvs[]>>
-      drule ltree_wbisim_bind_conv>>strip_tac>>gvs[]>>
-      qmatch_goalsub_abbrev_tac ‘_ >>= Y’>>
-      first_x_assum $ qspec_then ‘Y’ assume_tac>>
-      irule_at Any itree_wbisim_trans>>
-      first_x_assum $ irule_at Any>>
-      imp_res_tac ltree_lift_state_lift'>>gvs[]>>
-      fs[Abbr‘Y’]>>
-      fs[mrec_sem_simps,ltree_lift_cases]>>
-      TRY (fs[Once itree_wbisim_cases]>>NO_TAC)
-      (* SOME Error *)
-      >- (drule_then rev_drule ltree_lift_corres_evaluate_error>>
-          strip_tac>>gvs[]>>
-          drule_then rev_drule wbisim_Ret_unique>>strip_tac>>gvs[]>>
-          gvs[mrec_sem_simps,ltree_lift_cases]>>
-          fs[Once itree_wbisim_cases])>>
-      first_x_assum $ irule>>
-      gvs[Once evaluate_def])
-  (* Return *)
-  >- (gvs[AllCaseEqs(),h_prog_rule_return_def,h_prog_def,
-          panPropsTheory.eval_upd_clock_eq]>>
-      rpt CASE_TAC>>
-      gvs[mrec_sem_simps,ltree_lift_cases]>>
-      fs[Once itree_wbisim_cases])
-  (* Raise *)
-  >- (gvs[AllCaseEqs(),h_prog_rule_raise_def,h_prog_def,
-          panPropsTheory.eval_upd_clock_eq]>>
-      rpt CASE_TAC>>
-      gvs[mrec_sem_simps,ltree_lift_cases]>>
-      fs[Once itree_wbisim_cases])
-  (* Call *)
-  >- (simp[Once mrec_sem_Call_simps]>>
-      gvs[panPropsTheory.eval_upd_clock_eq,
-          panPropsTheory.opt_mmap_eval_upd_clock_eq1]>>
-      TOP_CASE_TAC>>
-      fs[mrec_sem_simps,ltree_lift_cases]>>
-      TRY (fs[Once itree_wbisim_cases]>>NO_TAC)>>
-      rpt CASE_TAC>>
-      fs[mrec_sem_simps,ltree_lift_cases]>>
-      TRY (fs[Once itree_wbisim_cases]>>NO_TAC)>>
-      Cases_on ‘s.clock = 0’>>gvs[]>>
-      FULL_CASE_TAC>>gvs[]>>
-      FULL_CASE_TAC>>gvs[]>>
-      FULL_CASE_TAC>>gvs[]>>
-      TRY (FULL_CASE_TAC>>gvs[])>>
-      TRY (FULL_CASE_TAC>>gvs[])>>
-      TRY (FULL_CASE_TAC>>gvs[])>>
-      TRY (FULL_CASE_TAC>>gvs[]>>
-           FULL_CASE_TAC>>gvs[]>>
-           TRY (FULL_CASE_TAC>>gvs[]))>>
-      gvs[ltree_lift_monad_law,set_var_defs,empty_locals_defs]>>
-      rpt (pairarg_tac>>gvs[])>>
-      ‘∀x. (dec_clock x).ffi = x.ffi’ by simp[dec_clock_def]>>fs[]>>
-      TRY (drule_then rev_drule ltree_lift_corres_evaluate>>
-           strip_tac>>gvs[])>>
-      TRY (drule_then rev_drule ltree_lift_corres_evaluate_error>>
-           strip_tac>>gvs[])>>
-      drule_then rev_drule wbisim_Ret_unique>>strip_tac>>gvs[]>>
-      imp_res_tac ltree_lift_state_lift'>>gvs[]>>
-      drule ltree_wbisim_bind_conv>>strip_tac>>gvs[]>>
-      qmatch_goalsub_abbrev_tac ‘_ >>= Y’>>
-      first_x_assum $ qspec_then ‘Y’ assume_tac>>
-      irule_at Any itree_wbisim_trans>>
-      first_x_assum $ irule_at Any>>
-      imp_res_tac ltree_lift_state_lift'>>gvs[]>>
-      fs[Abbr‘Y’]>>
-      fs[mrec_sem_simps,ltree_lift_cases,h_handle_call_ret_def]>>
-      TRY (CASE_TAC>>gvs[])>>
-      TRY (CASE_TAC>>gvs[])>>
-      gvs[mrec_sem_simps,ltree_lift_cases,set_var_defs]>>
-      TRY (simp[Once itree_wbisim_cases]>>NO_TAC)>>
-      metis_tac[])>>
-  (* ExtCall *)
-  gvs[AllCaseEqs(),h_prog_rule_ext_call_def,h_prog_def,
-      panPropsTheory.eval_upd_clock_eq]>>
-  rpt (CASE_TAC>>
-       fs[mrec_sem_simps,ltree_lift_cases,
-          msem_lift_monad_law,ltree_lift_monad_law])>>
-  TRY (fs[Once itree_wbisim_cases]>>NO_TAC)>>
-  pairarg_tac>>gvs[]>>
-  CASE_TAC>>
-  fs[Once itree_wbisim_cases]
+  rpt strip_tac >>
+  spose_not_then strip_assume_tac >>
+  Cases_on ‘evaluate (prog,reclock s with clock := k)’ >>
+  rename1 ‘_ = (res,st)’ >>
+  Cases_on ‘res = SOME Error’ >> gvs[]
+  >-  (imp_res_tac ltree_lift_corres_evaluate_error >>
+       gvs[]) >>
+  imp_res_tac ltree_lift_corres_evaluate >>
+  gvs[]
 QED
 
-Theorem evaluate_stree_trace_lub':
-  evaluate (prog:'a prog,reclock s with clock := k) = (SOME TimeOut,s') ∧
-  (∀p. ¬(ltree_lift query_oracle s.ffi (mrec_sem (h_prog (prog,s))) ≈ Ret p)) ∧
+Theorem nonret_imp_timeout':
   good_dimindex (:α) ∧
-  LPREFIX (fromList s'.ffi.io_events)
-          (fromList s.ffi.io_events
-           ++ₗ  stree_trace query_oracle event_filter s.ffi
-                (to_stree (mrec_sem (h_prog (prog,s))))) ∧
-  LPREFIX (fromList s'.ffi.io_events) ub ⇒
-  LPREFIX
-  (fromList s.ffi.io_events
-   ++ₗ  stree_trace query_oracle event_filter s.ffi
-        (to_stree (mrec_sem (h_prog (prog,s))))) ub
+  (∀p. ¬(ltree_lift query_oracle (s:('a,'b) state).ffi (mrec_sem (h_prog (prog,t))) ≈ Ret p)) ∧ t.ffi = s.ffi ⇒
+    ∃s'. evaluate (prog:'a prog, reclock t with clock := k) = (SOME TimeOut,s')
 Proof
   strip_tac>>
-  qabbrev_tac ‘x=reclock s with clock :=k’>>
-  ‘s.ffi = x.ffi’ by simp[Abbr‘x’]>>fs[]>>
-  Cases_on ‘evaluate(prog,x)’>>fs[]>>
-  ‘s = unclock x’ by simp[Abbr‘x’]>>gvs[]>>
-  qhdtm_x_assum ‘Abbrev’ kall_tac>>fs[]>>
-    rpt (pop_assum mp_tac)>>
-  MAP_EVERY qid_spec_tac [‘r’,‘x’,‘prog’]>>
-  completeInduct_on ‘x.clock’>>simp[PULL_FORALL]>>
-  simp[Once SWAP_FORALL_THM]>>
-  (*  recInduct evaluate_ind>>rw[]>>fs[Once evaluate_def]>>*)
-  Induct_on ‘prog’>>rw[]>>
-  (*  fs[Once LPREFIX_APPEND]>>*)
-  TRY(fs[Once evaluate_def]>>
-      rpt (pairarg_tac>>gvs[])>>gvs[]>>
-      TRY (drule panPropsTheory.evaluate_io_events_mono>>strip_tac)>>
-      simp[GSYM LAPPEND_fromList]>>
-      simp[Once LAPPEND_ASSOC]>>
-      simp[LFINITE_fromList, LAPPEND11_FINITE1]>>
-      TRY (gvs[AllCaseEqs()]>>rpt (pairarg_tac>>gvs[])>>NO_TAC))
-  >- (* Dec *)
-   (fs[h_prog_def,h_prog_rule_dec_def,mrec_sem_simps,ltree_lift_cases,
-       msem_lift_monad_law,to_stree_simps,stree_trace_simps,to_stree_monad_law,
-       panPropsTheory.eval_upd_clock_eq,ltree_lift_monad_law,AllCaseEqs()]>>
-    pairarg_tac>>gvs[]>>
-    fs[mrec_sem_simps,ltree_lift_cases,to_stree_simps,ltree_lift_monad_law,
-       stree_trace_simps,to_stree_monad_law,msem_lift_monad_law]>>
-    fs[msem_lift_monad_law,ltree_lift_monad_law,to_stree_monad_law]>>
-    first_x_assum $ qspecl_then [‘x with locals := x.locals |+ (m,value)’,‘st’] assume_tac>>
-    gvs[]>>
-    qmatch_asmsub_abbrev_tac ‘¬(X >>= Y ≈ _)’>>
-    Cases_on ‘∃w. X ≈ Ret w’
-    >- (fs[Abbr‘X’]>>
-        drule_then drule (iffLR ret_bind_nonret)>>strip_tac>>
-        Cases_on ‘w’>>fs[Abbr‘Y’]>>
-        fs[mrec_sem_simps,ltree_lift_cases]>>
-        fs[Once itree_wbisim_cases])>>
-    fs[Abbr‘X’]>>
-    drule (INST_TYPE [delta|->alpha] ltree_lift_nonret_bind_stree)>>
-    strip_tac>>gvs[)
-  >- (* Seq *)
-   (Cases_on ‘res’>>rpt (pairarg_tac>>gvs[])
-    >- (drule_then drule ltree_lift_corres_evaluate>>strip_tac>>fs[]>>
-        fs[h_prog_def,h_prog_rule_seq_def,mrec_sem_simps,ltree_lift_cases,
-           msem_lift_monad_law,to_stree_simps,stree_trace_simps,
-           to_stree_monad_law,
-           panPropsTheory.eval_upd_clock_eq,ltree_lift_monad_law]>>
-        imp_res_tac ltree_lift_state_lift'>>fs[]>>
-        drule_then drule (iffLR ret_bind_nonret)>>strip_tac>>
-        imp_res_tac stree_trace_ret_events'>>gvs[]>>
-        imp_res_tac (INST_TYPE [delta|->alpha] stree_trace_bind_append)>>
-        fs[mrec_sem_simps,ltree_lift_cases,to_stree_simps,
-           stree_trace_simps]>>
-        fs[PULL_FORALL]>>
-        drule evaluate_clock>>strip_tac>>
-        fs[LESS_OR_EQ]
-          >- (last_x_assum $ qspecl_then [‘s1’,‘prog'’,‘r’] assume_tac>>gvs[]>>
-              simp[Once (GSYM LAPPEND_ASSOC)]>>
-              pop_assum irule>>
-              simp[Once (LAPPEND_ASSOC)])>>
-        first_x_assum $ qspecl_then [‘s1’,‘r’] assume_tac>>gvs[]>>
-              simp[Once (GSYM LAPPEND_ASSOC)]>>
-              pop_assum irule>>
-        simp[Once (LAPPEND_ASSOC)])>>gvs[]>>
-    fs[h_prog_def,h_prog_rule_seq_def,mrec_sem_simps,ltree_lift_cases,
-       to_stree_simps,stree_trace_simps,panPropsTheory.eval_upd_clock_eq]>>
-    gvs[msem_lift_monad_law,ltree_lift_monad_law,to_stree_monad_law]>>
-    qmatch_asmsub_abbrev_tac ‘¬(X >>= Y ≈ _)’>>
-    Cases_on ‘∃w. X ≈ Ret w’
-    >- (fs[Abbr‘X’]>>
-        drule_then drule (iffLR ret_bind_nonret)>>strip_tac>>
-        Cases_on ‘w’>>
-        imp_res_tac ltree_lift_state_lift'>>fs[]>>
-        fs[Abbr‘Y’]>>
-        fs[mrec_sem_simps,ltree_lift_cases]>>
-        rename1 ‘Ret (q,r')’>>Cases_on ‘q’>>gvs[]>>
-        fs[mrec_sem_simps,ltree_lift_cases]>>
-        TRY (fs[Once itree_wbisim_cases]>>NO_TAC)>>
-        imp_res_tac stree_trace_ret_events'>>gvs[]>>
-        drule_then drule (iffLR ret_bind_nonret)>>strip_tac>>
-        gvs[]>>
-        fs[mrec_sem_simps,ltree_lift_cases]>>
-        imp_res_tac (INST_TYPE [delta|->alpha] stree_trace_bind_append)>>gvs[]>>
-        gvs[mrec_sem_simps,ltree_lift_cases,to_stree_simps,stree_trace_simps]>>
-        fs[PULL_FORALL]>>
-        ‘(reclock r').clock = x.clock ∨ (reclock r').clock < x.clock’
-          by simp[reclock_def]
-        >- (first_x_assum $ qspecl_then [‘reclock r'’,‘r’] assume_tac>>gvs[]>>
-            simp[Once (GSYM LAPPEND_ASSOC)]>>
-            pop_assum irule>>
-            simp[Once (LAPPEND_ASSOC)]>>
-            (* nonret imp timeout *) cheat)>>
-        last_x_assum $ qspecl_then [‘reclock r'’,‘prog'’,‘r’] assume_tac>>gvs[]>>
-        simp[Once (GSYM LAPPEND_ASSOC)]>>
-        pop_assum irule>>
-        simp[Once (LAPPEND_ASSOC)]>>
-        (* nonret imp timeout *) cheat)>>
-    fs[Abbr‘X’]>>
-    imp_res_tac (INST_TYPE [delta|->alpha] ltree_lift_nonret_bind_stree)>>fs[])
-  >- (* If *)
-   (gvs[AllCaseEqs()]>>rpt (pairarg_tac>>gvs[])>>
-    fs[h_prog_def,h_prog_rule_cond_def,ltree_lift_cases,stree_trace_simps,
-       panPropsTheory.eval_upd_clock_eq,mrec_sem_simps,to_stree_simps]>>
-    FULL_CASE_TAC>>gvs[]>>metis_tac[])
-  >- (* While *)
-   (fs[Once mrec_sem_while_unfold,mrec_sem_simps,ltree_lift_cases,
-       to_stree_simps,stree_trace_simps,panPropsTheory.eval_upd_clock_eq,
-       ltree_lift_monad_law,to_stree_monad_law]>>
-    rewrite_tac[Once mrec_sem_while_unfold]>>
-    fs[panPropsTheory.eval_upd_clock_eq]>>
-    ‘∀x. (dec_clock x).ffi = x.ffi’ by simp[dec_clock_def]>>fs[]>>
-    ntac 4 (TOP_CASE_TAC>>fs[])>>
-    fs[mrec_sem_simps,ltree_lift_cases,to_stree_simps,stree_trace_simps]>>
-    fs[bool_case_eq,empty_locals_defs]>>
-    gvs[PULL_FORALL]
-    >- cheat>>
-    Cases_on ‘res’>>gvs[]
-    >- (last_x_assum $ qspecl_then [‘s1’,‘While e prog’,‘r’] assume_tac>>gvs[]>>
-        rev_drule evaluate_clock>>simp[dec_clock_def]>>strip_tac>>gvs[]>>
-        simp[to_stree_monad_law]>>
-        
-        drule_then drule ltree_lift_corres_evaluate>>strip_tac>>fs[]>>
-        imp_res_tac ltree_lift_state_lift'>>fs[dec_clock_def]>>
-        fs[msem_lift_monad_law,ltree_lift_monad_law]>>gvs[]>>
-        drule_then drule (iffLR ret_bind_nonret)>>strip_tac>>
-        gvs[mrec_sem_simps,ltree_lift_cases]>>
-        imp_res_tac stree_trace_ret_events'>>gvs[]>>
-        imp_res_tac (INST_TYPE [delta|->alpha] stree_trace_bind_append)>>
-        fs[mrec_sem_simps,ltree_lift_cases,to_stree_simps,
-           stree_trace_simps]>>
-        simp[Once (GSYM LAPPEND_ASSOC)]>>
-        first_x_assum irule>>
-        fs[to_stree_simps,stree_trace_simps,to_stree_monad_law]>>
-        fs[Once (GSYM LAPPEND_ASSOC)])>>
-    rename1 ‘evaluate _ = (SOME xx,_)’>>Cases_on ‘xx’>> 
-   fs[msem_lift_monad_law,ltree_lift_monad_law,to_stree_monad_law]
-    >- (qmatch_asmsub_abbrev_tac ‘¬(X >>= Y ≈ _)’>>
-        Cases_on ‘∃w. X ≈ Ret w’
-        >- (fs[Abbr‘X’]>>
-            drule_then drule (iffLR ret_bind_nonret)>>strip_tac>>
-            Cases_on ‘w’>>fs[Abbr‘Y’]>>
-            fs[mrec_sem_simps,ltree_lift_cases]>>
-            imp_res_tac ltree_lift_state_lift'>>fs[]>>
-            rename1 ‘Ret (q,r')’>>Cases_on ‘q’>>
-            fs[mrec_sem_simps,ltree_lift_cases]
-            >- (
-(***)
-         qspecl_then [‘x’,‘r'’,‘dec_clock x’,‘NONE’,‘prog’] assume_tac(GEN_ALL ltree_Ret_to_evaluate')>>
-         gvs[]>>
-         qspecl_then [‘prog’,‘dec_clock x’,‘k-(dec_clock x).clock’] assume_tac(panPropsTheory.evaluate_add_clock_io_events_mono)>>
-         ‘(dec_clock x).clock < k’ by
-           (CCONTR_TAC>>fs[NOT_LESS]>>
-            drule panPropsTheory.evaluate_add_clock_eq>>
-            disch_then $ qspec_then ‘(dec_clock x).clock-k’ assume_tac>>
-            gvs[]>>
-            ‘(dec_clock x with clock := (dec_clock x).clock) = dec_clock x’
-              by simp[state_component_equality]>>fs[])>>
-          gvs[]>>
-
-            imp_res_tac stree_trace_ret_events'>>gvs[]>>
-          pop_assum $ assume_tac o GSYM>>
-          imp_res_tac (INST_TYPE [delta|->alpha] stree_trace_bind_append)>>gvs[]>>
-            gvs[to_stree_simps,stree_trace_simps]>>
-            gvs[IS_PREFIX_APPEND]>>
-            gvs[GSYM LAPPEND_fromList,LPREFIX_APPEND,LAPPEND_ASSOC,
-                LAPPEND11_FINITE1,LFINITE_fromList]>>
-            last_x_assum $ qspecl_then [‘reclock r'’,‘While e prog’,‘r’] assume_tac>>gvs[]>>
-            gvs[GSYM LAPPEND_fromList,LPREFIX_APPEND,LAPPEND_ASSOC,
-                LAPPEND11_FINITE1,LFINITE_fromList]>>
-         pop_assum irule>>
-         cheat (* the same *))>>
-            rename1 ‘Ret (SOME xx,_)’>>Cases_on ‘xx’>>
-            gvs[mrec_sem_simps,ltree_lift_cases]>>
-            TRY (fs[Once itree_wbisim_cases]>>NO_TAC)>>
-            fs[msem_lift_monad_law,ltree_lift_monad_law,to_stree_monad_law]>>
-            qspecl_then [‘x’,‘r'’,‘dec_clock x’,‘SOME Continue’,‘prog’] assume_tac(GEN_ALL ltree_Ret_to_evaluate')>>
-            gvs[]>>
-         qspecl_then [‘prog’,‘dec_clock x’,‘k-(dec_clock x).clock’] assume_tac(panPropsTheory.evaluate_add_clock_io_events_mono)>>
-         ‘(dec_clock x).clock < k’ by
-           (CCONTR_TAC>>fs[NOT_LESS]>>
-            drule panPropsTheory.evaluate_add_clock_eq>>
-            disch_then $ qspec_then ‘(dec_clock x).clock-k’ assume_tac>>
-            gvs[]>>
-            ‘(dec_clock x with clock := (dec_clock x).clock) = dec_clock x’
-              by simp[state_component_equality]>>fs[])>>
-          gvs[]>>
-            imp_res_tac stree_trace_ret_events'>>gvs[]>>
-          pop_assum $ assume_tac o GSYM>>
-          imp_res_tac (INST_TYPE [delta|->alpha] stree_trace_bind_append)>>gvs[]>>
-            gvs[to_stree_simps,stree_trace_simps]>>
-            gvs[IS_PREFIX_APPEND]>>
-            gvs[GSYM LAPPEND_fromList,LPREFIX_APPEND,LAPPEND_ASSOC,
-                LAPPEND11_FINITE1,LFINITE_fromList]>>
-            last_x_assum $ qspecl_then [‘reclock r'’,‘While e prog’,‘r’] assume_tac>>gvs[]>>
-            gvs[GSYM LAPPEND_fromList,LPREFIX_APPEND,LAPPEND_ASSOC,
-                LAPPEND11_FINITE1,LFINITE_fromList]>>
-            pop_assum irule>>
-            cheat (* the same *))>>
-        fs[Abbr‘X’]>>
-        last_x_assum $ qspecl_then [‘dec_clock x’,‘prog’,‘s1’] assume_tac>>gvs[]>>
-        imp_res_tac (INST_TYPE [delta|->alpha] ltree_lift_nonret_bind_stree)>>
-        fs[dec_clock_def])>>
-    
-
-)
-                  
-                       
-        
-
-
-
-TRY (fs[Once itree_wbisim_cases]>>NO_TAC)>>
-
-
-
-
-
-        rev_drule evaluate_clock>>simp[dec_clock_def]>>strip_tac>>gvs[]>>
-        simp[to_stree_monad_law]>>
-        
-        drule_then drule ltree_lift_corres_evaluate>>strip_tac>>fs[]>>
-        imp_res_tac ltree_lift_state_lift'>>fs[dec_clock_def]>>
-        fs[msem_lift_monad_law,ltree_lift_monad_law]>>gvs[]>>
-        drule_then drule (iffLR ret_bind_nonret)>>strip_tac>>
-        gvs[mrec_sem_simps,ltree_lift_cases]>>
-        imp_res_tac stree_trace_ret_events'>>gvs[]>>
-        imp_res_tac (INST_TYPE [delta|->alpha] stree_trace_bind_append)>>
-        fs[mrec_sem_simps,ltree_lift_cases,to_stree_simps,
-           stree_trace_simps]>>
-        simp[Once (GSYM LAPPEND_ASSOC)]>>
-        first_x_assum irule>>
-        fs[to_stree_simps,stree_trace_simps,to_stree_monad_law]>>
-        fs[Once (GSYM LAPPEND_ASSOC)])>>
-    rena
-
-
-fs[ltree_lift_monad_law,msem_lift_monad_law]>>
-    qmatch_asmsub_abbrev_tac ‘¬(X >>= Y ≈ _)’>>
-    Cases_on ‘∃w. X ≈ Ret w’
-        >- (fs[Abbr‘X’]>>
-            drule_then drule (iffLR ret_bind_nonret)>>strip_tac>>
-            Cases_on ‘w’>>fs[Abbr‘Y’]>>
-            fs[mrec_sem_simps,ltree_lift_cases]>>
-            imp_res_tac ltree_lift_state_lift'>>fs[]>>
-            rename1 ‘Ret (q,r')’>>Cases_on ‘q’>>
-            fs[mrec_sem_simps,ltree_lift_cases]>>
-            TRY (fs[Once itree_wbisim_cases]>>NO_TAC)>>
-            drule_then drule ltree_Ret_to_evaluate'>>gvs[]>>strip_tac>>
-            
-
-
-
-   )
-   cheat
-  >- (* Call *)
-   cheat
-   >>~- ([‘ShMem’],
-         gvs[AllCaseEqs()]>>rpt (pairarg_tac>>gvs[])>>
-         fs[h_prog_def,h_prog_rule_sh_mem_def,mrec_sem_simps,ltree_lift_cases,
-            to_stree_simps,stree_trace_simps,ltree_lift_monad_law,
-         panPropsTheory.opt_mmap_eval_upd_clock_eq1,set_var_defs,
-         panPropsTheory.eval_upd_clock_eq,to_stree_monad_law]>>
-         Cases_on ‘m’>>fs[sh_mem_op_def,sh_mem_load_def,sh_mem_store_def]>>
-         rpt (FULL_CASE_TAC>>gvs[]))>>
-  gvs[AllCaseEqs()]>>rpt (pairarg_tac>>gvs[])>>
-  fs[h_prog_def,empty_locals_defs,mrec_sem_simps,to_stree_simps,
-     stree_trace_simps,LAPPEND_NIL_2ND]
+  irule nonret_imp_timeout>>gvs[]
 QED
 
-
-
-
-Theorem evaluate_stree_trace_lub:
-  evaluate (prog:'a prog,reclock s with clock := k) = (SOME TimeOut,s') ∧
-  (∀p. ¬(ltree_lift query_oracle s.ffi (mrec_sem (h_prog (prog,s))) ≈ Ret p)) ∧
-  good_dimindex (:α) ∧
-  LPREFIX (fromList s'.ffi.io_events)
-          (fromList s.ffi.io_events
-           ++ₗ  stree_trace query_oracle event_filter s.ffi
-                (to_stree (mrec_sem (h_prog (prog,s))))) ∧
-  LPREFIX (fromList s'.ffi.io_events) ub ⇒
-  LPREFIX
-  (fromList s.ffi.io_events
-   ++ₗ  stree_trace query_oracle event_filter s.ffi
-        (to_stree (mrec_sem (h_prog (prog,s))))) ub
+Theorem nonret_imp_spin:
+  ∀f st t.
+    (∀p. ¬(ltree_lift f st t ≈ Ret p)) ⇒
+    ltree_lift f st t = spin
 Proof
-  strip_tac>>
-  qabbrev_tac ‘x=reclock s with clock :=k’>>
-  ‘s.ffi = x.ffi’ by simp[Abbr‘x’]>>fs[]>>
-  Cases_on ‘evaluate(prog,x)’>>fs[]>>
-  ‘s = unclock x’ by simp[Abbr‘x’]>>gvs[]>>
-  qhdtm_x_assum ‘Abbrev’ kall_tac>>fs[]>>
-  rpt (pop_assum mp_tac)>>
-  MAP_EVERY qid_spec_tac [‘s’,‘k’,‘r’,‘q’,‘x’, ‘prog’]>>
-  recInduct evaluate_ind>>rw[]>>fs[Once evaluate_def]>>
-  rpt (pairarg_tac>>gvs[])>>gvs[]>>
-  TRY (drule panPropsTheory.evaluate_io_events_mono>>strip_tac)>>
-(*  fs[Once LPREFIX_APPEND]>>*)
-  simp[GSYM LAPPEND_fromList]>>
-  simp[Once LAPPEND_ASSOC]>>
-  simp[LFINITE_fromList, LAPPEND11_FINITE1]>>
-  TRY (gvs[AllCaseEqs()]>>rpt (pairarg_tac>>gvs[])>>NO_TAC)
-  >- (* Dec *)
-   (fs[LPREFIX_APPEND]>>
-    fs[h_prog_def,h_prog_rule_dec_def,mrec_sem_simps,ltree_lift_cases,
-       msem_lift_monad_law,to_stree_simps,stree_trace_simps,to_stree_monad_law,
-       panPropsTheory.eval_upd_clock_eq,ltree_lift_monad_law,AllCaseEqs()]>>
-    pairarg_tac>>gvs[]>>
-    fs[mrec_sem_simps,ltree_lift_cases,to_stree_simps,ltree_lift_monad_law,
-       stree_trace_simps,to_stree_monad_law,msem_lift_monad_law]>>
-    fs[msem_lift_monad_law,ltree_lift_monad_law,to_stree_monad_law]>>
-    qmatch_asmsub_abbrev_tac ‘¬(X >>= Y ≈ _)’>>
-    Cases_on ‘∃w. X ≈ Ret w’
-    >- (fs[Abbr‘X’]>>
-        drule_then drule (iffLR ret_bind_nonret)>>strip_tac>>
-        Cases_on ‘w’>>fs[Abbr‘Y’]>>
-        fs[mrec_sem_simps,ltree_lift_cases]>>
-        fs[Once itree_wbisim_cases])>>
-    fs[Abbr‘X’]>>
-    drule (INST_TYPE [delta|->alpha] ltree_lift_nonret_bind_stree)>>
-    strip_tac>>gvs[]>>
-    fs[Once LAPPEND_ASSOC]>>
-    gvs[LFINITE_fromList, LAPPEND11_FINITE1]>>
-    metis_tac[])
-  (* ShMem *)
-   >>~- ([‘ShMem’],
-         gvs[LPREFIX_APPEND,AllCaseEqs()]>>rpt (pairarg_tac>>gvs[])>>
-         fs[h_prog_def,h_prog_rule_sh_mem_def,mrec_sem_simps,ltree_lift_cases,
-            to_stree_simps,stree_trace_simps,ltree_lift_monad_law,
-         panPropsTheory.opt_mmap_eval_upd_clock_eq1,set_var_defs,
-         panPropsTheory.eval_upd_clock_eq,to_stree_monad_law]>>
-         Cases_on ‘op’>>fs[sh_mem_op_def,sh_mem_load_def,sh_mem_store_def]>>
-         rpt (FULL_CASE_TAC>>gvs[]))
-  >- (* Seq *)
-   (fs[h_prog_def,h_prog_rule_seq_def,mrec_sem_simps,ltree_lift_cases,
-       msem_lift_monad_law,to_stree_simps,stree_trace_simps,
-       to_stree_monad_law,LPREFIX_APPEND,
-       panPropsTheory.eval_upd_clock_eq,ltree_lift_monad_law]>>
-    qmatch_asmsub_abbrev_tac ‘¬(X >>= Y ≈ _)’>>
-    Cases_on ‘∃w. X ≈ Ret w’
-    >- (fs[Abbr‘X’]>>
-        Cases_on ‘w’>>
-        drule_then drule ltree_Ret_to_evaluate'>>gvs[]>>strip_tac>>
-        imp_res_tac ltree_lift_state_lift'>>fs[]>>
-        drule_then drule (iffLR ret_bind_nonret)>>strip_tac>>
-        fs[Abbr‘Y’]>>
-        fs[mrec_sem_simps,ltree_lift_cases]>>
-        rename1 ‘Ret (q,r')’>>Cases_on ‘q’>>gvs[]>>
-        fs[mrec_sem_simps,ltree_lift_cases]>>
-        TRY (fs[Once itree_wbisim_cases]>>NO_TAC)>>
-        Cases_on ‘res’>>gvs[]
-        >- (
-
-(* the case of res = SOME TimeOut & itree for c1 is Ret *) cheat
-         drule_then drule ltree_Ret_to_evaluate'>>gvs[]>>strip_tac>>
-        qspecl_then [‘c1’,‘s’,‘k-s.clock’] assume_tac(panPropsTheory.evaluate_add_clock_io_events_mono)>>
-        ‘s.clock < k’ by
-          (CCONTR_TAC>>fs[NOT_LESS]>>
-           drule panPropsTheory.evaluate_add_clock_eq>>
-           disch_then $ qspec_then ‘s.clock-k’ assume_tac>>gvs[]>>
-           ‘s with clock := s.clock = s’ by
-             simp[state_component_equality]>>fs[])>>
-        gvs[]>>
-        imp_res_tac stree_trace_ret_events'>>gvs[]>>
-        drule_then drule (iffLR ret_bind_nonret)>>strip_tac>>
-        gvs[]>>
-        fs[mrec_sem_simps,ltree_lift_cases]>>
-
-   (Cases_on ‘res’>>gvs[]
-    >- (drule_then drule ltree_lift_corres_evaluate>>strip_tac>>fs[]>>
-        fs[h_prog_def,h_prog_rule_seq_def,mrec_sem_simps,ltree_lift_cases,
-           msem_lift_monad_law,to_stree_simps,stree_trace_simps,
-           to_stree_monad_law,LPREFIX_APPEND,
-           panPropsTheory.eval_upd_clock_eq,ltree_lift_monad_law]>>
-        imp_res_tac ltree_lift_state_lift'>>fs[]>>
-        drule_then drule (iffLR ret_bind_nonret)>>strip_tac>>
-        gvs[mrec_sem_simps,ltree_lift_cases]>>
-        imp_res_tac stree_trace_ret_events'>>gvs[]>>
-        imp_res_tac (INST_TYPE [delta|->alpha] stree_trace_bind_append)>>
-        fs[mrec_sem_simps,ltree_lift_cases,to_stree_simps,
-           stree_trace_simps]>>
-        gvs[IS_PREFIX_APPEND]>>
-        gvs[Once LAPPEND_ASSOC]>>
-        gvs[GSYM LAPPEND_fromList]>>
-        gvs[LFINITE_fromList, LAPPEND11_FINITE1]>>
-        gvs[Once (GSYM LAPPEND_ASSOC)]>>
-        metis_tac[])>>
-    fs[h_prog_def,h_prog_rule_seq_def,mrec_sem_simps,ltree_lift_cases,
-       msem_lift_monad_law,to_stree_simps,stree_trace_simps,
-       to_stree_monad_law,
-       panPropsTheory.eval_upd_clock_eq,ltree_lift_monad_law]>>
-    qmatch_asmsub_abbrev_tac ‘¬(X >>= Y ≈ _)’>>
-    Cases_on ‘∃w. X ≈ Ret w’
-    >- ((* the case of res = SOME TimeOut & itree for c1 is Ret *) cheat)
-       (*fs[Abbr‘X’]>>
-        drule_then drule (iffLR ret_bind_nonret)>>strip_tac>>
-        Cases_on ‘w’>>fs[Abbr‘Y’]>>
-        imp_res_tac ltree_lift_state_lift'>>fs[]>>
-        fs[mrec_sem_simps,ltree_lift_cases]>>
-        rename1 ‘Ret (q,r')’>>Cases_on ‘q’>>fs[]>>
-        fs[mrec_sem_simps,ltree_lift_cases]>>
-        TRY (fs[Once itree_wbisim_cases]>>NO_TAC)>>
-
-        drule_then drule ltree_Ret_to_evaluate'>>gvs[]>>strip_tac>>
-        qspecl_then [‘c1’,‘s’,‘k-s.clock’] assume_tac(panPropsTheory.evaluate_add_clock_io_events_mono)>>
-        ‘s.clock < k’ by
-          (CCONTR_TAC>>fs[NOT_LESS]>>
-           drule panPropsTheory.evaluate_add_clock_eq>>
-           disch_then $ qspec_then ‘s.clock-k’ assume_tac>>gvs[]>>
-           ‘s with clock := s.clock = s’ by
-             simp[state_component_equality]>>fs[])>>
-        gvs[]>>
-        drule panPropsTheory.evaluate_io_events_mono>>strip_tac>>fs[]>>
-        imp_res_tac stree_trace_ret_events'>>gvs[]>>
-        imp_res_tac (INST_TYPE [delta|->alpha] ltree_lift_nonret_bind_stree)>>
-        imp_res_tac (INST_TYPE [delta|->alpha] stree_trace_bind_append)>>gvs[]>>
-        gvs[mrec_sem_simps,ltree_lift_cases,
-           to_stree_simps,stree_trace_simps]>>
-        gvs[IS_PREFIX_APPEND]>>
-        fs[GSYM LAPPEND_fromList]>>
-        fs[Once LAPPEND_ASSOC]>>
-        fs[LFINITE_fromList, LAPPEND11_FINITE1]>>
-        fs[LPREFIX_fromList]>>
-        qpat_x_assum ‘LAPPEND _ _ = _’ $ assume_tac o GSYM >> fs[]>>
-        gvs[]>>
-        fs[LPREFIX_fromList]>>*)
-    fs[Abbr‘X’]>>
-    drule (INST_TYPE [delta|->alpha] ltree_lift_nonret_bind_stree)>>
-    strip_tac>>gvs[])
-  >- (* If *)
-   (gvs[AllCaseEqs()]>>rpt (pairarg_tac>>gvs[])>>
-    fs[h_prog_def,h_prog_rule_cond_def,ltree_lift_cases,stree_trace_simps,
-       panPropsTheory.eval_upd_clock_eq,mrec_sem_simps,to_stree_simps]>>
-    FULL_CASE_TAC>>gvs[]>>
-    fs[Once LAPPEND_ASSOC]>>
-    fs[LFINITE_fromList, LAPPEND11_FINITE1]>>
-    metis_tac[])
-  >- (* While *)
-   (completeInduct_on ‘s.clock’>>gvs[]>>rw[]>>
-
-    gvs[AllCaseEqs()]>>
-    gvs[IS_PREFIX_APPEND,dec_clock_def]>>
-    fs[Once mrec_sem_while_unfold]>>
-    gvs[mrec_sem_simps,ltree_lift_cases,
-         to_stree_simps,panPropsTheory.eval_upd_clock_eq,
-         stree_trace_simps,ltree_lift_monad_law,to_stree_monad_law]>>
-
-        ntac 2 strip_tac>>
-
-
-    
-
-qpat_x_assum ‘_ = (SOME TimeOut,_)’ mp_tac>>
-    TOP_CASE_TAC>>fs[]>>
-    TOP_CASE_TAC>>fs[]>>
-    TOP_CASE_TAC>>fs[]>>
-    TOP_CASE_TAC>>fs[]>>
-    TOP_CASE_TAC>>fs[]
-    >- (strip_tac>>gvs[empty_locals_defs]>>cheat (* False *))>>
-    CASE_TAC>>gvs[]
-    (* res = NONE *)
-    >- (strip_tac>>
-        last_x_assum mp_tac>>
-        qpat_x_assum ‘LPREFIX _ (LAPPEND _ (_ _ _ _ (_ (_ (h_prog (While e c,unclock s))))))’ mp_tac>>
-        once_rewrite_tac[mrec_sem_while_unfold]>>
-        simp[mrec_sem_simps,ltree_lift_cases,
-             to_stree_simps,panPropsTheory.eval_upd_clock_eq,
-             stree_trace_simps,ltree_lift_monad_law,to_stree_monad_law]>>
-        ntac 2 strip_tac>>
-    qmatch_asmsub_abbrev_tac ‘¬(X >>= Y ≈ _)’>>
-    Cases_on ‘∃w. X ≈ Ret w’
-        >- (fs[Abbr‘X’]>>
-            drule_then drule (iffLR ret_bind_nonret)>>strip_tac>>
-            Cases_on ‘w’>>fs[Abbr‘Y’]>>
-            fs[mrec_sem_simps,ltree_lift_cases]>>
-            imp_res_tac ltree_lift_state_lift'>>fs[]>>
-            rename1 ‘Ret (q,r')’>>Cases_on ‘q’>>
-            fs[mrec_sem_simps,ltree_lift_cases]>>
-            TRY (fs[Once itree_wbisim_cases]>>NO_TAC)>>
-
-
-        first_x_assum $ qspec_then ‘r’ mp_tac>>gvs[]>>
-        qpat_x_assum ‘_ = (NONE,_)’ assume_tac>>
-        drule_then drule ltree_lift_corres_evaluate>>strip_tac>>gvs[]>>
-        ‘∀x. (dec_clock x).ffi = x.ffi’ by simp[dec_clock_def]>>fs[]>>
-        imp_res_tac ltree_lift_state_lift'>>gvs[]>>
-        impl_tac >-
-         (last_x_assum mp_tac>>
-          simp[Once mrec_sem_while_unfold]>>
-          simp[mrec_sem_simps,ltree_lift_cases,
-               to_stree_simps,panPropsTheory.eval_upd_clock_eq,
-               stree_trace_simps,ltree_lift_monad_law,to_stree_monad_law]>>
-          strip_tac>>
-          drule_then drule (iffLR ret_bind_nonret)>>strip_tac>>
-          gvs[mrec_sem_simps,ltree_lift_cases,
-              stree_trace_simps,ltree_lift_monad_law,to_stree_monad_law])>>
-        impl_tac >-
-         (
-         drule panPropsTheory.evaluate_io_events_mono>>strip_tac>>fs[]>>
-         gvs[IS_PREFIX_APPEND]>>
-
-
-qpat_x_assum ‘_ = (SOME _,_)’ mp_tac>>simp[Once evaluate_def])>>
-        strip_tac>>
-        simp[Once mrec_sem_while_unfold,mrec_sem_simps,ltree_lift_cases,
-             to_stree_simps,panPropsTheory.eval_upd_clock_eq,
-             stree_trace_simps,ltree_lift_monad_law,to_stree_monad_law]>>
-        imp_res_tac stree_trace_ret_events'>>gvs[]>>
-        imp_res_tac (INST_TYPE [delta|->alpha] stree_trace_bind_append)>>gvs[]>>
-        fs[mrec_sem_simps,ltree_lift_cases,to_stree_simps,
-           stree_trace_simps]>>
-        fs[Once LAPPEND_ASSOC]>>
-        metis_tac[])>>
-    (* res = SOME x *)
-    CASE_TAC>>gvs[]>>strip_tac>>gvs[]>>
-    ‘∀x. (dec_clock x).ffi = x.ffi’ by simp[dec_clock_def]>>fs[]
-    >- (fs[Once mrec_sem_while_unfold,mrec_sem_simps,ltree_lift_cases,
-           to_stree_simps,stree_trace_simps,panPropsTheory.eval_upd_clock_eq,
-           ltree_lift_monad_law,to_stree_monad_law]>>
-        qmatch_asmsub_abbrev_tac ‘X >>= Y’>>
-        Cases_on ‘∃p. X ≈ Ret p’
-        >-
-         (fs[Abbr‘X’]>>
-          Cases_on ‘p’>>rename1 ‘Ret (q,r')’>>
-          imp_res_tac ltree_lift_state_lift'>>fs[]>>
-         qspecl_then [‘s’,‘r'’,‘dec_clock s’,‘q’,‘c’] assume_tac(GEN_ALL ltree_Ret_to_evaluate')>>
-         gvs[]>>
-         qspecl_then [‘c’,‘dec_clock s’,‘k-(dec_clock s).clock’] assume_tac(panPropsTheory.evaluate_add_clock_io_events_mono)>>
-         ‘(dec_clock s).clock < k’ by
-           (CCONTR_TAC>>fs[NOT_LESS]>>
-            drule panPropsTheory.evaluate_add_clock_eq>>
-            disch_then $ qspec_then ‘(dec_clock s).clock-k’ assume_tac>>
-            gvs[]>>
-            ‘(dec_clock s with clock := (dec_clock s).clock) = dec_clock s’
-              by simp[state_component_equality]>>fs[])>>
-          gvs[]>>
-          drule_then drule (iffLR ret_bind_nonret)>>strip_tac>>
-          fs[Abbr‘Y’]>>Cases_on ‘q’>>
-          gvs[mrec_sem_simps,ltree_lift_cases]>>
-          imp_res_tac stree_trace_ret_events'>>gvs[]>>
-          pop_assum $ assume_tac o GSYM>>
-          imp_res_tac (INST_TYPE [delta|->alpha] stree_trace_bind_append)>>gvs[]>>
-          gvs[to_stree_simps,stree_trace_simps]>>
-          simp[GSYM LAPPEND_ASSOC]>>
-          fs[IS_PREFIX_APPEND]>>
-          simp[GSYM LAPPEND_fromList]>>
-          simp[LAPPEND_ASSOC]>>metis_tac[])>>
-        fs[Abbr‘X’]>>
-        drule (INST_TYPE [delta|->alpha] ltree_lift_nonret_bind_stree)>>
-        strip_tac>>gvs[]>>metis_tac[])>>
-    last_x_assum $ qspec_then ‘r’ mp_tac>>gvs[]>>
-    qpat_x_assum ‘_ = (SOME Continue,_)’ assume_tac>>
-    drule_then drule ltree_lift_corres_evaluate>>strip_tac>>gvs[]>>
-    imp_res_tac ltree_lift_state_lift'>>gvs[]>>
-    impl_tac >-
-     (last_x_assum mp_tac>>
-      simp[Once mrec_sem_while_unfold]>>
-      simp[mrec_sem_simps,ltree_lift_cases,
-           to_stree_simps,panPropsTheory.eval_upd_clock_eq,
-           stree_trace_simps,ltree_lift_monad_law,to_stree_monad_law]>>
-      strip_tac>>
-      drule_then drule (iffLR ret_bind_nonret)>>strip_tac>>
-      gvs[mrec_sem_simps,ltree_lift_cases,
-          stree_trace_simps,ltree_lift_monad_law,to_stree_monad_law])>>
-    impl_tac >-
-     (qpat_x_assum ‘_ = (SOME TimeOut,_)’ mp_tac>>simp[Once evaluate_def])>>
-    strip_tac>>
-    simp[Once mrec_sem_while_unfold,mrec_sem_simps,ltree_lift_cases,
-         to_stree_simps,panPropsTheory.eval_upd_clock_eq,
-         stree_trace_simps,ltree_lift_monad_law,to_stree_monad_law]>>
-    imp_res_tac stree_trace_ret_events'>>gvs[]>>
-    imp_res_tac (INST_TYPE [delta|->alpha] stree_trace_bind_append)>>gvs[]>>
-    fs[mrec_sem_simps,ltree_lift_cases,to_stree_simps,
-       stree_trace_simps]>>
-    fs[Once LAPPEND_ASSOC]>>
-    metis_tac[])
-cheat
-  >~[‘Tick’]
-  >- (gvs[AllCaseEqs()]>>rpt (pairarg_tac>>gvs[])>>
-      fs[h_prog_def,empty_locals_defs,mrec_sem_simps,to_stree_simps,
-         stree_trace_simps,LAPPEND_NIL_2ND])>>
-(* Call *)
-  gvs[AllCaseEqs()]>>rpt (pairarg_tac>>gvs[])
-  >- (fs[empty_locals_defs]>>metis_tac[])
-  >- (fs[Once mrec_sem_Call_simps,
-         panPropsTheory.eval_upd_clock_eq,
-         panPropsTheory.opt_mmap_eval_upd_clock_eq1]>>
-      fs[to_stree_simps,stree_trace_simps,ltree_lift_cases,
-         ltree_lift_monad_law,to_stree_monad_law]>>
-      ‘(dec_clock s).ffi = s.ffi’ by simp[dec_clock_def]>>fs[]>>
-      qmatch_asmsub_abbrev_tac ‘X >>= Y’>>
-      Cases_on ‘∃p. X ≈ Ret p’
-      >-(fs[Abbr‘X’]>>Cases_on ‘p’>>rename1 ‘Ret (q,r')’>>
-         imp_res_tac ltree_lift_state_lift'>>fs[]>>
-         drule_then drule (iffLR ret_bind_nonret)>>strip_tac>>
-         Cases_on ‘q’>>gvs[Abbr‘Y’]>>
-         gvs[mrec_sem_simps,ltree_lift_cases,h_handle_call_ret_def]>>
-         TRY (fs[Once itree_wbisim_cases]>>NO_TAC)>>
-         rename1 ‘Ret (SOME xx,r')’>>Cases_on ‘xx’>>
-         gvs[mrec_sem_simps,ltree_lift_cases,h_handle_call_ret_def]>>
-         TRY (fs[Once itree_wbisim_cases]>>NO_TAC)
-         (* Return *)
-         >- (rpt (FULL_CASE_TAC>>
-                  gvs[mrec_sem_simps,ltree_lift_cases])>>
-             fs[Once itree_wbisim_cases])>>
-         (* Exception *)
-         rpt (FULL_CASE_TAC>>
-              gvs[mrec_sem_simps,ltree_lift_cases])>>
-         TRY (fs[Once itree_wbisim_cases]>>NO_TAC)>>
-         gvs[set_var_defs]>>
-         imp_res_tac (INST_TYPE [delta|->alpha] stree_trace_bind_append)>>gvs[]>>
-         qspecl_then [‘s’,‘r'’,‘dec_clock s with locals := newlocals’,‘SOME (Exception m v)’,‘prog’] assume_tac(GEN_ALL ltree_Ret_to_evaluate')>>
-         gvs[]>>
-         qspecl_then [‘prog’,‘dec_clock s with locals := newlocals’,‘k-(dec_clock s).clock’] assume_tac(panPropsTheory.evaluate_add_clock_io_events_mono)>>
-         ‘(dec_clock s).clock < k’ by
-           (CCONTR_TAC>>fs[NOT_LESS]>>
-            drule panPropsTheory.evaluate_add_clock_eq>>
-            disch_then $ qspec_then ‘(dec_clock s).clock-k’ assume_tac>>
-            gvs[]>>
-            ‘(dec_clock s with clock := (dec_clock s).clock) = dec_clock s’
-              by simp[state_component_equality]>>fs[])>>
-         gvs[h_handle_call_ret_def]>>
-         gvs[mrec_sem_simps,ltree_lift_cases,set_var_defs,
-             to_stree_simps,stree_trace_simps]>>
-         drule panPropsTheory.evaluate_io_events_mono>>strip_tac>>fs[]>>
-         gvs[IS_PREFIX_APPEND,empty_locals_defs]>>
-         imp_res_tac stree_trace_ret_events'>>gvs[]>>
-         qpat_assum ‘_ ++ _ = _ ++ _’ $ assume_tac o GSYM>>fs[]>>
-         fs[GSYM LAPPEND_fromList]>>
-         fs[Once (GSYM LAPPEND_ASSOC)]>>
-         qpat_x_assum ‘LAPPEND _ _ = LAPPEND _ _’ $ assume_tac o GSYM >> fs[]>>
-         fs[Once LAPPEND_ASSOC]>>metis_tac[])>>
-      gvs[Abbr‘X’]>>
-      drule (INST_TYPE [delta|->alpha] ltree_lift_nonret_bind_stree)>>
-      strip_tac>>gvs[empty_locals_defs]>>metis_tac[])>>
-  (* RetCall *)
-  fs[Once mrec_sem_Call_simps,set_var_defs,
-     panPropsTheory.eval_upd_clock_eq,
-     panPropsTheory.opt_mmap_eval_upd_clock_eq1]>>
-  fs[to_stree_simps,stree_trace_simps,ltree_lift_cases,
-     ltree_lift_monad_law,to_stree_monad_law]>>
-  ‘(dec_clock s).ffi = s.ffi’ by simp[dec_clock_def]>>fs[]>>
-  drule_then rev_drule ltree_lift_corres_evaluate>>strip_tac>>gvs[]>>
-  imp_res_tac ltree_lift_state_lift'>>gvs[]>>
-  imp_res_tac stree_trace_ret_events'>>gvs[]>>
-  imp_res_tac (INST_TYPE [delta|->alpha] stree_trace_bind_append)>>gvs[]>>
-  drule_then drule (iffLR ret_bind_nonret)>>strip_tac>>
-  fs[to_stree_simps,stree_trace_simps,ltree_lift_cases,
-     ltree_lift_monad_law,to_stree_monad_law]>>
-  gvs[h_handle_call_ret_def]>>
-  gvs[mrec_sem_simps,ltree_lift_cases,set_var_defs,
-      to_stree_simps,stree_trace_simps]>>
-  fs[Once LAPPEND_ASSOC]>>metis_tac[]
-  >- (
-  >>cheat
+  rpt strip_tac >>
+  CONV_TAC SYM_CONV >>
+  rw[Once itree_bisimulation] >>
+  qexists ‘CURRY {(spin, ltree_lift f st t) | (∀p. ¬(ltree_lift f st t ≈ Ret p))}’ >>
+  conj_tac >- (rw[EXISTS_PROD] >> metis_tac[]) >>
+  pop_assum kall_tac >>
+  rw[] >>
+  gvs[UNCURRY_eq_pair]
+  >- (qpat_x_assum ‘_ = spin’ mp_tac >> rw[Once spin])
+  >- (rename1 ‘ltree_lift f st t’ >>
+      Cases_on ‘t’ >>
+      gvs[ltree_lift_cases,itree_wbisim_neq]
+      >- (qpat_x_assum ‘_ = spin’ mp_tac >> rw[Once spin] >> metis_tac[])
+      >- (Cases_on ‘a’ >> gvs[ltree_lift_cases,UNCURRY_eq_pair,PULL_EXISTS] >>
+          pairarg_tac >>
+          gvs[] >>
+          qpat_x_assum ‘_ = spin’ mp_tac >> rw[Once spin] >>
+          metis_tac[]))
+  >- (qpat_x_assum ‘_ = spin’ mp_tac >> rw[Once spin])
 QED
+
+(*** divergence ***)
 
 Theorem evaluate_stree_trace_LPREFIX:
   evaluate (prog:'a prog,reclock s with clock := k) = (SOME TimeOut,s') ∧
@@ -4086,7 +3225,7 @@ Proof
   recInduct evaluate_ind>>rw[]>>fs[Once evaluate_def]>>
   rpt (pairarg_tac>>gvs[])>>gvs[]>>
   TRY (drule panPropsTheory.evaluate_io_events_mono>>strip_tac)>>
-(*  fs[LPREFIX_APPEND]>> (* why APPEND?? *)*)
+  fs[LPREFIX_APPEND]>> (* why APPEND?? *)
   TRY (simp[GSYM LAPPEND_fromList]>>
        simp[Once LAPPEND_ASSOC]>>
        simp[LFINITE_fromList, LAPPEND11_FINITE1]>>
@@ -4119,12 +3258,7 @@ fs[h_prog_def,h_prog_rule_dec_def,mrec_sem_simps,ltree_lift_cases,
          Cases_on ‘op’>>fs[sh_mem_op_def,sh_mem_load_def,sh_mem_store_def]>>
          rpt (FULL_CASE_TAC>>gvs[]))
   >- (* Seq *)
-   (rpt $ pop_assum mp_tac>>
-    MAP_EVERY qid_spec_tac [‘s’, ‘s1’, ‘res’]>>
-    completeInduct_on ‘s.clock’>>rw[]
-    imp_res_tac evaluate_clock>>
-
-    gvs[AllCaseEqs()]>>rpt (pairarg_tac>>gvs[])
+   (gvs[AllCaseEqs()]>>rpt (pairarg_tac>>gvs[])
     >- (drule_then drule ltree_lift_corres_evaluate>>strip_tac>>fs[]>>
         fs[h_prog_def,h_prog_rule_seq_def,mrec_sem_simps,ltree_lift_cases,
            msem_lift_monad_law,to_stree_simps,stree_trace_simps,
@@ -4136,25 +3270,14 @@ fs[h_prog_def,h_prog_rule_dec_def,mrec_sem_simps,ltree_lift_cases,
         imp_res_tac (INST_TYPE [delta|->alpha] stree_trace_bind_append)>>
         fs[mrec_sem_simps,ltree_lift_cases,to_stree_simps,
            stree_trace_simps]>>
-        gvs[Once LAPPEND_ASSOC]>>
-        gvs[Once LAPPEND_ASSOC])>>
-
+        gvs[Once LAPPEND_ASSOC]>>metis_tac[])>>
     fs[h_prog_def,h_prog_rule_seq_def,mrec_sem_simps,ltree_lift_cases,
        to_stree_simps,stree_trace_simps,panPropsTheory.eval_upd_clock_eq]>>
     fs[msem_lift_monad_law,ltree_lift_monad_law,to_stree_monad_law]>>
-    qmatch_asmsub_abbrev_tac ‘¬(X >>= Y ≈ _)’>>
+    qmatch_asmsub_abbrev_tac ‘X >>= Y’>>
     Cases_on ‘∃w. X ≈ Ret w’
-    >- (fs[Abbr‘X’]>>
-        drule_then drule (iffLR ret_bind_nonret)>>strip_tac>>
-        Cases_on ‘w’>>
-        imp_res_tac ltree_lift_state_lift'>>fs[]>>
-        fs[Abbr‘Y’]>>
-        fs[mrec_sem_simps,ltree_lift_cases]>>
-        rename1 ‘Ret (q,r')’>>Cases_on ‘q’>>gvs[]>>
-        fs[mrec_sem_simps,ltree_lift_cases]>>
-        TRY (fs[Once itree_wbisim_cases]>>NO_TAC)>>
-
-         drule_then drule ltree_Ret_to_evaluate'>>gvs[]>>strip_tac>>
+    >- (fs[Abbr‘X’]>>Cases_on ‘w’>>
+        drule_then drule ltree_Ret_to_evaluate'>>gvs[]>>strip_tac>>
         qspecl_then [‘c1’,‘s’,‘k-s.clock’] assume_tac(panPropsTheory.evaluate_add_clock_io_events_mono)>>
         ‘s.clock < k’ by
           (CCONTR_TAC>>fs[NOT_LESS]>>
@@ -4165,9 +3288,6 @@ fs[h_prog_def,h_prog_rule_dec_def,mrec_sem_simps,ltree_lift_cases,
         gvs[]>>
         imp_res_tac stree_trace_ret_events'>>gvs[]>>
         drule_then drule (iffLR ret_bind_nonret)>>strip_tac>>
-        gvs[]>>
-        fs[mrec_sem_simps,ltree_lift_cases]>>
-
         fs[Abbr‘Y’]>>
         imp_res_tac (INST_TYPE [delta|->alpha] ltree_lift_nonret_bind_stree)>>
         imp_res_tac ltree_lift_state_lift'>>fs[]>>
@@ -4176,6 +3296,7 @@ fs[h_prog_def,h_prog_rule_dec_def,mrec_sem_simps,ltree_lift_cases,
         fs[GSYM LAPPEND_fromList]>>
         fs[Once LAPPEND_ASSOC]>>
         fs[LFINITE_fromList, LAPPEND11_FINITE1]>>
+        simp[LPREFIX_fromList]>>
         qpat_x_assum ‘LAPPEND _ _ = _’ $ assume_tac o GSYM >> fs[]>>
         fs[Once LAPPEND_ASSOC]>>metis_tac[])>>
     fs[Abbr‘X’]>>
@@ -4236,16 +3357,16 @@ fs[h_prog_def,h_prog_rule_dec_def,mrec_sem_simps,ltree_lift_cases,
          (fs[Abbr‘X’]>>
           Cases_on ‘p’>>rename1 ‘Ret (q,r')’>>
           imp_res_tac ltree_lift_state_lift'>>fs[]>>
-         qspecl_then [‘s’,‘r'’,‘dec_clock s’,‘q’,‘c’] assume_tac(GEN_ALL ltree_Ret_to_evaluate')>>
-         gvs[]>>
-         qspecl_then [‘c’,‘dec_clock s’,‘k-(dec_clock s).clock’] assume_tac(panPropsTheory.evaluate_add_clock_io_events_mono)>>
-         ‘(dec_clock s).clock < k’ by
-           (CCONTR_TAC>>fs[NOT_LESS]>>
-            drule panPropsTheory.evaluate_add_clock_eq>>
-            disch_then $ qspec_then ‘(dec_clock s).clock-k’ assume_tac>>
-            gvs[]>>
-            ‘(dec_clock s with clock := (dec_clock s).clock) = dec_clock s’
-              by simp[state_component_equality]>>fs[])>>
+          qspecl_then [‘dec_clock s’,‘r'’,‘unclock (dec_clock s)’,‘q’,‘c’] assume_tac(GEN_ALL ltree_Ret_to_evaluate')>>
+          gvs[]>>
+          qspecl_then [‘c’,‘dec_clock s’,‘k-(dec_clock s).clock’] assume_tac(panPropsTheory.evaluate_add_clock_io_events_mono)>>
+          ‘(dec_clock s).clock < k’ by
+            (CCONTR_TAC>>fs[NOT_LESS]>>
+             drule panPropsTheory.evaluate_add_clock_eq>>
+             disch_then $ qspec_then ‘(dec_clock s).clock-k’ assume_tac>>
+             gvs[]>>
+             ‘(dec_clock s with clock := (dec_clock s).clock) = dec_clock s’
+               by simp[dec_clock_def,state_component_equality]>>fs[])>>
           gvs[]>>
           drule_then drule (iffLR ret_bind_nonret)>>strip_tac>>
           fs[Abbr‘Y’]>>Cases_on ‘q’>>
@@ -4321,7 +3442,7 @@ fs[h_prog_def,h_prog_rule_dec_def,mrec_sem_simps,ltree_lift_cases,
          TRY (fs[Once itree_wbisim_cases]>>NO_TAC)>>
          gvs[set_var_defs]>>
          imp_res_tac (INST_TYPE [delta|->alpha] stree_trace_bind_append)>>gvs[]>>
-         qspecl_then [‘s’,‘r'’,‘dec_clock s with locals := newlocals’,‘SOME (Exception m v)’,‘prog’] assume_tac(GEN_ALL ltree_Ret_to_evaluate')>>
+         qspecl_then [‘dec_clock s’,‘r'’,‘unclock (dec_clock s) with locals := newlocals’,‘SOME (Exception m v)’,‘prog’] assume_tac(GEN_ALL ltree_Ret_to_evaluate')>>
          gvs[]>>
          qspecl_then [‘prog’,‘dec_clock s with locals := newlocals’,‘k-(dec_clock s).clock’] assume_tac(panPropsTheory.evaluate_add_clock_io_events_mono)>>
          ‘(dec_clock s).clock < k’ by
@@ -4365,48 +3486,225 @@ fs[h_prog_def,h_prog_rule_dec_def,mrec_sem_simps,ltree_lift_cases,
   fs[Once LAPPEND_ASSOC]>>metis_tac[]
 QED
 
-Theorem nonret_imp_timeout:
-  ∀s r s' prog:'a prog k.
-    good_dimindex (:α) ∧
-    (∀p. ¬(ltree_lift query_oracle s.ffi (mrec_sem (h_prog (prog,s))) ≈ Ret p)) ⇒
-    ∃s'. evaluate (prog,reclock s with clock := k) = (SOME TimeOut,s')
+Theorem LUB_LAPPEND_fromList:
+  lprefix_chain X ∧ X ≠ ∅ ⇒
+  LAPPEND (fromList l) (LUB X)
+  = LUB {LAPPEND (fromList l) l' | l' | l' ∈ X}
 Proof
-  rpt strip_tac >>
-  spose_not_then strip_assume_tac >>
-  Cases_on ‘evaluate (prog,reclock s with clock := k)’ >>
-  rename1 ‘_ = (res,st)’ >>
-  Cases_on ‘res = SOME Error’ >> gvs[]
-  >-  (imp_res_tac ltree_lift_corres_evaluate_error >>
-       gvs[]) >>
-  imp_res_tac ltree_lift_corres_evaluate >>
-  gvs[]
+  strip_tac>>
+  simp[lprefix_lubTheory.build_lprefix_lub_def]>>
+  simp[LNTH_EQ]>>
+  qid_spec_tac ‘l’>>
+  simp[Once SWAP_FORALL_THM]>>
+  Induct>>strip_tac
+  (* 0 *)
+  >- (simp[LNTH_LUNFOLD,LNTH_LAPPEND]>>
+      Cases_on ‘l’>>fs[]>>
+      simp[lprefix_lubTheory.build_lprefix_lub_f_def]>>
+      simp[PULL_EXISTS]>>
+      irule lprefix_lubTheory.exists_lprefix_chain_nth>>
+      rw[PULL_EXISTS]>- fs[PULL_EXISTS,MEMBER_NOT_EMPTY]>>
+      fs[lprefix_chain_def]>>rw[]>>
+      gvs[LPREFIX_fromList,LPREFIX_LCONS])>>
+  (* SUC n *)
+  rpt strip_tac>>gvs[LNTH_LAPPEND]>>
+  IF_CASES_TAC>>gvs[LNTH_THM,NOT_LESS]
+  (* SUC n < LENGTH l *)
+  >- (Cases_on ‘l’>>gvs[]>>
+      first_x_assum $ qspec_then ‘t’ assume_tac>>gvs[]>>
+      CASE_TAC>>gvs[]
+      >- (pop_assum mp_tac>>
+          fs[lprefix_lubTheory.build_lprefix_lub_f_def]>>
+          fs[lprefix_chain_nth_def]>>
+          DEEP_INTRO_TAC some_intro>>simp[]>>
+          rpt strip_tac>>gvs[]>>
+          fs[PULL_FORALL]>>
+          fs[GSYM MEMBER_NOT_EMPTY])>>
+      gvs[LNTH_fromList]>>
+      CASE_TAC>>gvs[]>>
+      qmatch_asmsub_abbrev_tac ‘Y = SOME (q,r)’>>
+      ‘Y = SOME (1,h)’
+        by (simp[Abbr‘Y’]>>
+            pop_assum mp_tac>>
+            fs[lprefix_lubTheory.build_lprefix_lub_f_def]>>
+            fs[lprefix_chain_nth_def]>>
+            DEEP_INTRO_TAC some_intro>>simp[]>>
+            rpt strip_tac>>gvs[])>>gvs[]>>
+      irule (iffLR LNTH_EQ)>>
+      simp[Once LUNFOLD_BISIMULATION]>>
+      qexists ‘CURRY {(n,SUC n) | n | T}’>>
+      rw[]>>
+      pop_assum mp_tac>>
+      fs[lprefix_lubTheory.build_lprefix_lub_f_def]>>
+      fs[lprefix_chain_nth_def]>>
+      DEEP_INTRO_TAC some_intro>>simp[PULL_EXISTS]>>
+      DEEP_INTRO_TAC some_intro>>simp[PULL_EXISTS]>>
+      DEEP_INTRO_TAC some_intro>>simp[PULL_EXISTS])>>
+  (* LENGTH l ≤ SUC n *)
+  gvs[]>>
+  CASE_TAC>>fs[]
+  >- (pop_assum mp_tac>>
+      fs[lprefix_lubTheory.build_lprefix_lub_f_def]>>
+      fs[lprefix_chain_nth_def]>>
+      DEEP_INTRO_TAC some_intro>>simp[]>>
+      rpt strip_tac>>gvs[]>>
+      simp[Once LUNFOLD]>>
+      rpt CASE_TAC>>gvs[]>>
+      pop_assum mp_tac>>
+      fs[lprefix_lubTheory.build_lprefix_lub_f_def]>>
+      fs[lprefix_chain_nth_def]>>
+      DEEP_INTRO_TAC some_intro>>simp[]>>
+      rpt strip_tac>>gvs[]>>
+      Cases_on ‘l’>>gvs[])>>
+  CASE_TAC>>fs[]>>
+  pop_assum mp_tac>>
+  fs[lprefix_lubTheory.build_lprefix_lub_f_def]>>
+  fs[lprefix_chain_nth_def]>>
+  DEEP_INTRO_TAC some_intro>>simp[]>>
+  rpt strip_tac>>gvs[LNTH_LAPPEND,LNTH_fromList]>>
+  Cases_on ‘l’>>gvs[]
+  >- (rpt CASE_TAC>>gvs[]>>
+      pop_assum mp_tac>>
+      fs[lprefix_lubTheory.build_lprefix_lub_f_def]>>
+      fs[lprefix_chain_nth_def]>>
+      DEEP_INTRO_TAC some_intro>>simp[]>>
+      rpt strip_tac>>gvs[LNTH_LAPPEND,LNTH_fromList])>>
+  first_x_assum $ qspec_then ‘t’ assume_tac>>gvs[]>>
+  irule (iffLR LNTH_EQ)>>
+  simp[Once LUNFOLD_BISIMULATION]>>
+  qexists ‘CURRY {(n,SUC n) | n | T}’>>
+  rw[]>>
+  fs[lprefix_lubTheory.build_lprefix_lub_f_def]>>
+  fs[lprefix_chain_nth_def]>>
+  DEEP_INTRO_TAC some_intro>>simp[PULL_EXISTS]>>
+  DEEP_INTRO_TAC some_intro>>simp[PULL_EXISTS]>>
+  rpt strip_tac>>
+  gvs[PULL_FORALL,LNTH_fromList,LNTH_LAPPEND]>>
+  rpt CASE_TAC>>gvs[MEMBER_NOT_EMPTY,NOT_LESS]>>
+  qexistsl [‘x’,‘l'''’]>>gvs[]>>
+  rpt strip_tac>>gvs[lprefix_chain_def]>>
+  last_x_assum $ qspecl_then [‘l'''’,‘l''''’] assume_tac>>
+  gvs[llistTheory.LPREFIX_NTH]>>
+  first_x_assum $ qspec_then ‘y1 - LENGTH t’ assume_tac>>gvs[]
 QED
 
-Theorem nonret_imp_spin:
-  ∀f st t.
-    (∀p. ¬(ltree_lift f st t ≈ Ret p)) ⇒
-    ltree_lift f st t = spin
+Definition stree_trace2_def:
+  stree_trace2 f p fs ^st =
+  LMAP THE $
+  LFILTER IS_SOME $
+  LUNFOLD
+  (λ(fs',t). case t of
+                 Ret r => NONE
+               | Tau u => SOME ((fs',u),NONE)
+               | Vis e k => let (a,rbytes,fs'') = f fs' e in
+                              if p a then
+                                SOME ((fs'',k a),SOME (make_io_event e rbytes))
+                              else
+                                SOME ((fs'', k a),NONE))
+  (fs,st)
+End
+
+Theorem stree_trace_simp:
+  stree_trace q f ffi st =
+  (case st of
+     Ret _ => [||]
+   | Tau u => stree_trace q f ffi u
+   | Vis a g => let (a',rbytes,fs'') = q ffi a in
+                  if f a'
+                  then
+                    make_io_event a rbytes:::
+                                  stree_trace q f fs'' (g a')
+                  else stree_trace q f fs'' (g a'))
 Proof
-  rpt strip_tac >>
-  CONV_TAC SYM_CONV >>
-  rw[Once itree_bisimulation] >>
-  qexists ‘CURRY {(spin, ltree_lift f st t) | (∀p. ¬(ltree_lift f st t ≈ Ret p))}’ >>
-  conj_tac >- (rw[EXISTS_PROD] >> metis_tac[]) >>
-  pop_assum kall_tac >>
-  rw[] >>
-  gvs[UNCURRY_eq_pair]
-  >- (qpat_x_assum ‘_ = spin’ mp_tac >> rw[Once spin])
-  >- (rename1 ‘ltree_lift f st t’ >>
-      Cases_on ‘t’ >>
-      gvs[ltree_lift_cases,itree_wbisim_neq]
-      >- (qpat_x_assum ‘_ = spin’ mp_tac >> rw[Once spin] >> metis_tac[])
-      >- (Cases_on ‘a’ >> gvs[ltree_lift_cases,UNCURRY_eq_pair,PULL_EXISTS] >>
-          pairarg_tac >>
-          gvs[] >>
-          qpat_x_assum ‘_ = spin’ mp_tac >> rw[Once spin] >>
-          metis_tac[]))
-  >- (qpat_x_assum ‘_ = spin’ mp_tac >> rw[Once spin])
+  simp[stree_trace_def]>>
+  simp[Once LUNFOLD]>>
+  Cases_on ‘st’>>gvs[]>>
+  rpt (pairarg_tac>>fs[])>>
+  CASE_TAC>>gvs[]
 QED
+
+Theorem stree_trace2_simp:
+  stree_trace2 q f ffi st =
+  (case st of
+     Ret _ => [||]
+   | Tau u => stree_trace2 q f ffi u
+   | Vis a g => let (a',rbytes,fs'') = q ffi a in
+                  if f a'
+                  then
+                    make_io_event a rbytes:::
+                                  stree_trace2 q f fs'' (g a')
+                  else stree_trace2 q f fs'' (g a'))
+Proof
+  simp[stree_trace2_def]>>
+  simp[Once LUNFOLD]>>
+  Cases_on ‘st’>>gvs[]>>
+  rpt (pairarg_tac>>fs[])>>
+  CASE_TAC>>gvs[]
+QED
+
+Theorem stree_trace2_ok:
+  stree_trace q f ffi st = stree_trace2 q f ffi st
+Proof
+  simp[Once stree_trace_simp,Once stree_trace2_simp]>>
+  simp[Once LLIST_BISIMULATION0]>>
+  qexists ‘CURRY
+         {((case st of
+            Ret v => [||]
+          | Tau u => stree_trace q f ffi u
+          | Vis a g =>
+            (λ(a',rbytes,fs'').
+                 if f a' then
+                   make_io_event a rbytes:::stree_trace q f fs'' (g a')
+                 else stree_trace q f fs'' (g a')) (q ffi a)),
+           case st of
+             Ret v => [||]
+           | Tau u => stree_trace2 q f ffi u
+           | Vis a g =>
+               (λ(a',rbytes,fs'').
+                  if f a' then
+                    make_io_event a rbytes:::stree_trace2 q f fs'' (g a')
+                  else stree_trace2 q f fs'' (g a')) (q ffi a))|st|T}’>>
+  rw[] >- metis_tac[]>>
+  Cases_on ‘st’
+  >- (disj1_tac>>simp[])
+  >- (Cases_on ‘stree_trace q f ffi u’>>fs[]
+      >-(fs[stree_trace_def]>>
+         fs[Once LUNFOLD]>>
+         Cases_on ‘u’>>gvs[Once stree_trace2_simp]
+
+
+
+>>gvs[]
+  >- (Cases_on ‘stree_trace q f ffi u’>>fs[]
+      >- (fs[Once stree_trace_simp,Once stree_trace2_simp]>>
+
+
+          >- (Casesdisj2_tac>>disj1_tac
+        
+  
+QED
+
+Theorem temp:
+  (∀k. FST (evaluate (prog,reclock s with clock := k)) = SOME TimeOut) ∧
+  (∀p. ¬(ltree_lift query_oracle s.ffi (mrec_sem (h_prog (prog,s))) ≈
+             Ret p)) ∧
+  good_dimindex (:α) ⇒
+  fromList s.ffi.io_events
+  ++ₗstree_trace query_oracle event_filter s.ffi
+                 (to_stree (mrec_sem (h_prog (prog,s)))) =
+  LUB (IMAGE
+       (λk. fromList (SND (evaluate (prog,reclock s with clock := k))).ffi.
+                    io_events) 𝕌(:num))
+Proof
+  strip_tac>>
+  simp[IMAGE_DEF]>>
+  simp[LNTH_EQ]>>
+  Induct>>simp[LNTH_LAPPEND,LNTH_fromList]
+  
+                               
+QED
+
+panPropsTheory.evaluate_add_clock_io_events_mono |> SIMP_RULE std_ss [IS_PREFIX_APPEND]
 
 (* Final goal:
 
@@ -4442,33 +3740,19 @@ Proof
           conj_asm2_tac
           >- (irule lprefix_lubTheory.lprefix_lub_is_chain>>metis_tac[])>>
           simp[lprefix_lubTheory.lprefix_lub_def]>>fs[]>>
-          conj_asm1_tac>>rpt strip_tac>>gvs[]
-          >- (gvs[PULL_EXISTS]>>
-              first_x_assum $ qspec_then ‘k’ assume_tac>>
+          conj_asm1_tac>>rpt strip_tac>>gvs[PULL_EXISTS]
+          >- (first_x_assum $ qspec_then ‘k’ assume_tac>>
               irule evaluate_stree_trace_LPREFIX>>gvs[]>>
               qmatch_asmsub_abbrev_tac ‘FST X’>>Cases_on ‘X’>>
               gvs[]>>metis_tac[])>>
           (* least upper bound *)
-          fs[LPREFIX_APPEND]>>
-          fs[PULL_FORALL]
-
-
-          last_x_assum $ qspec_then ‘k’ assume_tac>>
-          first_x_assum $ qspec_then ‘fromList (SND (evaluate (prog,reclock s with clock := k))).ffi.io_events’ assume_tac>>
-          first_x_assum $ qspec_then ‘fromList (SND (evaluate (prog,reclock s with clock := k))).ffi.io_events’ assume_tac>>
-          gvs[]>>
-
-          qmatch_goalsub_abbrev_tac ‘_ = LAPPEND X _’>>
-          ‘¬ (LFINITE X)’ by cheat>>
-          simp[NOT_LFINITE_APPEND]>>
-          fs[GSYM PULL_FORALL]
-          fs[LPREFIX_APPEND]
-
-
-rpt (first_x_assum $ qspec_then ‘k’ assume_tac)>>
-          irule evaluate_stree_trace_lub>>
-          qmatch_asmsub_abbrev_tac ‘FST X’>>Cases_on ‘X’>>
-          gvs[]>>metis_tac[])>>
+          ‘∀k. ∃s'. evaluate (prog, reclock s with clock := k) = (SOME TimeOut,s')’
+            by (strip_tac>>
+                last_x_assum $ qspec_then ‘k’ assume_tac>>
+                qpat_abbrev_tac ‘X = evaluate _’>>
+                Cases_on ‘X’>>gvs[])>>
+          drule_then drule lub2>>
+          strip_tac>>gvs[])
       (* False cases: ltree_lift converges and evalate diverges... *)
       simp [FORALL_PROD] >> rw [] >>
       spose_not_then kall_tac >>
